basicBugSet cleanup

Dafny/Common/GeneralNonInterferenceProperties.s.dfy
@@ -1,72 +1,80 @@
 include "System.s.dfy"
+include "../Libraries/Sets.i.dfy"
 
 abstract module GeneralNonInterferenceProperties {
         import opened System_s
+        import opened Collections__Sets_i
 
+
+    predicate RemovedBehaviors(b:System_s.behavior)
+    
     // Describes 'bad' behavior that a safe patch should prune
     predicate MiniSpec(b:System_s.behavior)
-    // {
-    //     exists s :: s in b && !s.ok
-    // }
+    {
+        RemovedBehaviors(b)
+    }
 
 // -- 
     // benignPatch: "The patch does not add any NEW behaviors"
-    predicate benignPatch(a:seq<System_s.behavior>,b:seq<System_s.behavior>)
+    predicate benignPatch(pre:set<System_s.behavior>,post:set<System_s.behavior>)
     {
-        // forall p :: p in b ==> p in a
-       
-        var aOut := allBehaviorOutput(a);
-        var bOut := allBehaviorOutput(b);
-        forall p :: p in bOut ==> p in aOut
-
+        var preOutput := allBehaviorOutputSet(pre);
+        var postOutput := allBehaviorOutputSet(post);
+        forall postB :: postB in postOutput ==> postB in preOutput
     }
 
-    // successfulPatch: "The patch prunes the BAD (defined by MiniSpec) behaviors"
-    predicate successfulPatch(b:seq<System_s.behavior>)
+    // // successfulPatch: "The patch prunes the BAD (defined by MiniSpec) behaviors" 
+    predicate successfulPatch(post:set<System_s.behavior>)
     {
-        forall p :: MiniSpec(p) ==> !(p in b)
-       
-    }    
-    // completePatch: "The patch preserves the GOOD behavior" // Name; complete -> preserving ? 
-    predicate completePatch(a:seq<System_s.behavior>,b:seq<System_s.behavior>)
+        forall postB :: MiniSpec(postB) ==> !(postB in post)
+    }
+
+    // // completePatch: "The patch preserves the GOOD behavior" // Name; complete -> preserving ? 
+    predicate completePatch(pre:set<System_s.behavior>,post:set<System_s.behavior>)
     {
         // forall p :: (p in a && !MiniSpec(p)) ==> p in b
 
-        var aOut := allBehaviorOutput(a);
-        var bOut := allBehaviorOutput(b);
-        forall p :: (behaviorOutput(p) in aOut && !MiniSpec(p)) ==> behaviorOutput(p) in bOut
+        var preOutput := allBehaviorOutputSet(pre);
+        var postOutput := allBehaviorOutputSet(post);
+        forall preB :: (behaviorOutput(preB) in preOutput && !MiniSpec(preB)) ==> behaviorOutput(preB) in postOutput
+    }
+    // completePatch: "The patch preserves the GOOD behavior" // Name; complete -> preserving ? 
+    predicate completePatchMS(pre:set<System_s.behavior>,post:set<System_s.behavior>)
+    {
+        // forall p :: (p in a && !MiniSpec(p)) ==> p in b
+        var preModMs := MakeSubset(pre, x => !MiniSpec(x));
+        var preModMsOut := allBehaviorOutputSet(preModMs);
+        var postOutput := allBehaviorOutputSet(post);
+        forall preB :: behaviorOutput(preB) in preModMsOut ==> behaviorOutput(preB) in postOutput
     }
 
-    //     // successfulPatch: "The patch prunes the BAD (defined by MiniSpec) behaviors"
-    // predicate successfulPatch_Restricted(a:seq<System_s.behavior>,b:seq<System_s.behavior>)
-    // {
-    //     // forall p :: p in a && MiniSpec(p) ==> !(p in b)
-    //     var aOut := allBehaviorOutput(a);
-    //     var bOut := allBehaviorOutput(b);
-    //     forall p :: (behaviorOutput(p) in aOut && MiniSpec(p)) ==> !(behaviorOutput(p) in bOut)
-
-    // }
     
-    // The conjuntion of benign, successful and complete imply that; that after apply the patch, b retains all good behavior from a and 
-    // is pruned of all bad behavior. 
-    predicate safePatch(a:seq<System_s.behavior>,b:seq<System_s.behavior>)
+    // // The conjuntion of benign, successful and complete imply that; that after apply the patch, b retains all good behavior from a and 
+    // // is pruned of all bad behavior. 
+
+    predicate safePatch(pre:set<System_s.behavior>,post:set<System_s.behavior>)
     {
         // forall p :: (p in a && !MiniSpec(p)) <==> p in b
-        var aOut := allBehaviorOutput(a);
-        var bOut := allBehaviorOutput(b);
-        forall p :: (behaviorOutput(p) in aOut && !MiniSpec(p)) <==> behaviorOutput(p) in bOut
+        var preOutput := allBehaviorOutputSet(pre);
+        var postOutput := allBehaviorOutputSet(post);
+        forall preB :: (behaviorOutput(preB) in preOutput && !MiniSpec(preB)) <==> behaviorOutput(preB) in postOutput
     }
 
-    lemma fullPatch(a:seq<System_s.behavior>,b:seq<System_s.behavior>)
-        requires benignPatch(a,b);
-        requires successfulPatch(b);
-        requires completePatch(a,b);
-        ensures safePatch(a,b);
-        // {
-        //     var aOut := allBehaviorOutput(a);
-        //     var bOut := allBehaviorOutput(b);
-        //     assert forall p :: (behaviorOutput(p) in aOut && !MiniSpec(p)) <==> behaviorOutput(p) in bOut;
-        // }
+    predicate safePatchMS(pre:set<System_s.behavior>,post:set<System_s.behavior>)
+    {           
+    //  forall p :: (p in a && !MiniSpec(p)) <==> p in b
+        var preModMs := MakeSubset(pre, x => !MiniSpec(x));
+        var preModMsOut := allBehaviorOutputSet(preModMs);
+        var postOutput := allBehaviorOutputSet(post);
+        forall preB :: behaviorOutput(preB) in preModMsOut <==> behaviorOutput(preB) in postOutput
+    } 
+
+    lemma fullPatch(pre:set<System_s.behavior>,post:set<System_s.behavior>)
+        requires benignPatch(pre,post);
+        requires successfulPatch(post);
+        requires completePatchMS(pre,post);
+        ensures safePatchMS(pre,post);
+
 
 
 //// Other General Functions
