Dafny/Common/System.s.dfy
@@ -1,12 +1,14 @@
 include "Types.s.dfy"
 include "Memory.s.dfy"
 include "../Libraries/Seqs.s.dfy"
+include "../Libraries/Sets.i.dfy"
 
  module System_s
 {
     import opened Types_s
     import opened Memory_s
-     import opened Collections__Seqs_s
+    import opened Collections__Seqs_s
+    import opened Collections__Sets_i
 
 //////////////
 
@@ -62,54 +64,20 @@ include "../Libraries/Seqs.s.dfy"
         |b| >= 2 && b == [b[0]] + evalCode(c,b[0])
     }
 
-    function behaviorOutput(b:behavior) : (bOut:seq<output>)
+function {:opaque} behaviorOutput(b:behavior) : (bOut:seq<output>)
         ensures |bOut| == |b| 
         ensures forall i :: (i >= 0 && i < |b|) ==> bOut[i] == b[i].o
+        decreases |b|
 
-
-    function allBehaviors(a:set<behavior>) : (bOut:set<seq<output>>)
+     function  allBehaviorOutputSet(bSet:set<behavior>) : (allBOut:set<seq<output>>)
         // ensures |bOut| == |a|
-        decreases |a|
-    {
-        if |a| == 0 then
-            var empty := {};
-            assert |empty| == |a|; 
-            empty
-        else   
-            var x :| x in a;
-            var a' := a - {x};
-            var singleton := {behaviorOutput(x)};
-            var s := singleton + allBehaviors(a');
-            
-            s
-            //{behaviorOutput(x)} + allBehaviors(a')
-    }
-
-    function allBehaviorOutput(a:seq<behavior>) : (bOut:seq<seq<output>>)
-        ensures |bOut| == |a|
-        ensures forall a' :: a' in a ==> behaviorOutput(a') in bOut;
-        ensures forall i :: (i >= 0 && i < |a|) ==> bOut[i] == behaviorOutput(a[i])
-        // ensures forall b :: behaviorOutput(b) in bOut ==> b in a;
-        // ensures forall b :: b in bOut ==> exists a' :: a' in a && behaviorOutput(a') == b
-        // ensures forall a' :: behaviorOutput(a') in bOut ==> a' in a;
-        // ensures forall b :: b in bOut ==> exists aa :: aa in a && behaviorOutput(aa) == b
-        decreases |a|
-    {
-        if |a| == 0 then
-            var out := [];
-            assert forall a' :: behaviorOutput(a') in out ==> a' in a;
-            out
-        else   
-            // var x :| x in a;
-            // var a' := a - {x};
-            // assert x in a;
-            var out := [behaviorOutput(a[0])] + allBehaviorOutput(all_but_first(a));
-            // assert behaviorOutput(a[0]) in out && a[0] in;
-            // assert forall b :: behaviorOutput(b) in [behaviorOutput(x)] ==> behaviorOutput(b) == behaviorOutput(x);
-            // assert forall b :: behaviorOutput(b) in [behaviorOutput(x)] ==> 
-            out
-            //{behaviorOutput(x)} + allBehaviors(a')
-    }
+        ensures SurjectiveOver(bSet,allBOut, x => behaviorOutput(x));
+        ensures forall b :: b in bSet ==> behaviorOutput(b) in allBOut;
+        ensures (allBOut == allBehaviorOutputSet(bSet)) ==> SurjectiveOver(bSet,allBOut, x => behaviorOutput(x));
+        ensures |bSet| > 0 ==> |allBOut| > 0
+        ensures |bSet| == 0 ==> |allBOut| == 0;
+        decreases |bSet|
+    
 
 
 
