Dafny/LLVM/behaviorLemmas.i.dfy
@@ -1,0 +1,182 @@
+include "./llvmREFACTOR.i.dfy"
+include "../Libraries/Seqs.s.dfy"
+include "../Libraries/Sets.i.dfy"
+
+
+module behavior_lemmas 
+{
+    import opened LLVM_defRE
+    import opened Collections__Sets_i
+    import opened Collections__Seqs_s
+
+
+    // type behavior = seq<state>
+    predicate ValidBehaviorNonTrivial(b:behavior)
+    {
+        ValidBehavior(b) && |b| > 0
+        
+    }
+    predicate {:opaque} BehaviorEvalsCode(c:codeRe,b:behavior)
+    {
+        |b| >= 2 && b == [b[0]] + evalCodeRE(c,b[0])
+    }
+
+    lemma behaviorThatEvalsSameCodeWithSameInitIsEqual(s:state,c:codeRe,b:behavior)
+        requires ValidState(s);
+        requires ValidBehaviorNonTrivial(b);
+        requires BehaviorEvalsCode(c,b);
+        ensures forall b' :: (|b'| > 0 && BehaviorEvalsCode(c,b')  && b'[0] == b[0]) ==> b' == b;
+     {  
+         reveal_BehaviorEvalsCode();
+         assert forall b' :: (|b'| > 0 && BehaviorEvalsCode(c,b')  && b'[0] == b[0]) ==> b' == b;
+     }
+
+
+    function {:opaque} behaviorOutput(b:behavior) : (bOut:seq<output>)
+        ensures |bOut| == |b| 
+        ensures forall i :: (i >= 0 && i < |b|) ==> bOut[i] == b[i].o
+        decreases |b|
+    {
+        if |b| == 0 then
+            []
+        else 
+            [b[0].o] + behaviorOutput(all_but_first(b))
+    }
+
+     function  allBehaviorOutputSet(bSet:set<behavior>) : (allBOut:set<seq<output>>)
+        // ensures |bOut| == |a|
+        ensures SurjectiveOver(bSet,allBOut, x => behaviorOutput(x));
+        ensures forall b :: b in bSet ==> behaviorOutput(b) in allBOut;
+        ensures (allBOut == allBehaviorOutputSet(bSet)) ==> SurjectiveOver(bSet,allBOut, x => behaviorOutput(x));
+        ensures |bSet| > 0 ==> |allBOut| > 0
+        ensures |bSet| == 0 ==> |allBOut| == 0;
+        decreases |bSet|
+    {
+        // reveal_SurjectiveOver();
+        reveal_behaviorOutput();
+        if |bSet| == 0 then
+            var out := {};
+            assert forall b :: behaviorOutput(b) in out ==> (exists elem :: elem in bSet && behaviorOutput(elem) == behaviorOutput(b));
+            allBehaviorsSetSurjective(bSet,out);
+            out
+        else   
+             var behavior :| behavior in bSet;
+             var bSubset := bSet - {behavior};
+             var singleOutput := {behaviorOutput(behavior)};
+             var rest := allBehaviorOutputSet(bSubset);
+             var out := singleOutput + rest;
+             subsetUnion(singleOutput,rest,behaviorOutput(behavior));
+             allBehaviorsSetSurjective(bSet,out);
+             out
+
+    }
+
+    predicate {:opaque} expandedAllBehaviorsSurjective(bSet:set<behavior>,allBOut:set<seq<output>>)
+    {
+        (forall y :: y in allBOut ==> (exists x :: x in bSet && behaviorOutput(x) == y))
+    }
+
+    lemma allBehaviorsSetSurjective(bSet:set<behavior>,allBOut:set<seq<output>>)
+        requires SurjectiveOver(bSet,allBOut, x => behaviorOutput(x));
+        ensures expandedAllBehaviorsSurjective(bSet,allBOut);
+        ensures (forall y :: y in allBOut ==> (exists x :: x in bSet && behaviorOutput(x) == y))
+    {
+         reveal_expandedAllBehaviorsSurjective();
+         assert expandedAllBehaviorsSurjective(bSet,allBOut);
+         assert  (forall y :: y in allBOut ==> (exists x :: x in bSet && behaviorOutput(x) == y));
+    }
+
+    lemma allBehaviorEqualityIsSurjective(bSet:set<behavior>,allBOut:set<seq<output>>)
+       requires allBOut == allBehaviorOutputSet(bSet);
+       ensures SurjectiveOver(bSet,allBOut, x => behaviorOutput(x));
+       ensures  SurjectiveOver(bSet,allBOut, x => behaviorOutput(x)) ==> (forall y :: y in allBOut ==> (exists x :: x in bSet && behaviorOutput(x) == y));    
+    {
+        reveal_behaviorOutput();
+        reveal_expandedAllBehaviorsSurjective();
+        assert SurjectiveOver(bSet,allBOut, x => behaviorOutput(x));
+        assert SurjectiveOver(bSet,allBOut, x => behaviorOutput(x)) ==> (forall y :: y in allBOut ==> (exists x :: x in bSet && behaviorOutput(x) == y));
+    //    allBehaviorsSetSurjective(bSet,allBOut);
+    //    assert (forall y :: y in allBOut ==> (exists x :: x in bSet && behaviorOutput(x) == y));
+    }
+
+    lemma subsetOfBehaviorImpliesSubsetOfOutput(superset:set<behavior>,subset:set<behavior>,f:behavior->bool)
+        requires subset == MakeSubset(superset,f);
+        ensures forall subsetOut :: subsetOut in allBehaviorOutputSet(subset) ==> subsetOut in allBehaviorOutputSet(superset);
+    {
+        assert forall subElem :: subElem in subset ==> subElem in superset;
+        var superOut := allBehaviorOutputSet(superset);
+        var subOut := allBehaviorOutputSet(subset);
+
+        assert forall subsetOut :: subsetOut in subOut ==> subsetOut in superOut;
+    }
+
+    lemma subsetOfBehaviorImpliesSubsetOfOutputFull(superset:set<behavior>,subset:set<behavior>,superOut:set<seq<output>>,subOut:set<seq<output>>,f:behavior->bool)
+        requires subset == MakeSubset(superset,f);
+        requires superOut == allBehaviorOutputSet(superset);
+        requires subOut == allBehaviorOutputSet(subset);
+
+        ensures forall subsetOut :: subsetOut in subOut ==> subsetOut in superOut;
+    {
+        assert forall subElem :: subElem in subset ==> subElem in superset;
+        assert forall subsetOut :: subsetOut in subOut ==> subsetOut in superOut;
+    }
+
+   
+    lemma identicalBehaviorSetsHaveSameOutput(a:set<behavior>,b:set<behavior>)
+        requires a == b
+        ensures allBehaviorOutputSet(a) == allBehaviorOutputSet(b)
+    {
+    }
+
+
+    predicate equalOutput(a:seq<output>,b:seq<output>)
+        ensures equalOutput(a,b) ==> (a == b)
+    {
+        && |a| == |b|
+        && forall i :: (i >=0 && i < |a|) ==> a[i] == b[i]
+    }
+
+
+    lemma equalOutputLemma(a:seq<output>,b:seq<output>)
+        requires equalOutput(a,b)
+        ensures a == b
+    {
+        assert a == b;
+    }
+
+    lemma outputIsEqual(a:seq<output>,b:seq<output>)
+        requires a == b
+        ensures equalOutput(a,b)
+    {
+        assert equalOutput(a,b);
+    }
+
+    lemma transitiveEquality(a:seq<output>,b:seq<output>,c:seq<output>)
+        requires equalOutput(a,c);
+        requires equalOutput(b,c);
+        ensures equalOutput(a,b);
+        ensures a == b
+    {
+        assert equalOutput(a,b);
+        equalOutputLemma(a,b);
+    }
+
+    lemma equalOutputIsTransitive(a:seq<output>,b:seq<output>,all:seq<seq<output>>)
+        requires a == b;
+        requires a in all;
+        ensures b in all;
+    {
+        assert b in all;
+    }
+
+lemma equalOutputIsTransitiveSet(a:seq<output>,b:seq<output>,all:set<seq<output>>)
+        requires a == b;
+        requires a in all;
+        ensures b in all;
+    {
+        assert b in all;
+    }
+
+
+}
+
