Dafny/examples/BasicBugSet/simpleBugProperties.i.dfy
@@ -6,6 +6,7 @@ include "../../LLVM/llvmREFACTOR.i.dfy"
 include "../../LLVM/types.dfy"
 include "../../Libraries/Seqs.s.dfy"
 include "../../Libraries/Sets.i.dfy"
+include "../../LLVM/behaviorLemmas.i.dfy"
 
 
 module simpleBugProperties{
@@ -17,6 +18,7 @@ module simpleBugProperties{
     import opened types
     import opened Collections__Seqs_s
     import opened Collections__Sets_i
+    import opened behavior_lemmas
 
 ///////////////////////////////
 
